Adding sum types.

reducibility/Convertibility.v
@@ -3,9 +3,16 @@ Require Import Setoid CMorphisms Term.
 Inductive reduction : term -> term -> Type :=
 | reduction_β : forall t u, reduction (app (lam t) u) (subs_term (CONS u ESID) t)
 | reduction_η : forall t, reduction (lam (app (lift_term (ELSHFT ELID) t) (var 0))) t
+| reduction_ι_l : forall t u1 u2, reduction (cse (lft t) u1 u2) (subs_term (CONS t ESID) u1)
+| reduction_ι_r : forall t u1 u2, reduction (cse (rgt t) u1 u2) (subs_term (CONS t ESID) u2)
 | reduction_lam : forall t r, reduction t r -> reduction (lam t) (lam r)
 | reduction_app_l : forall t u r, reduction t r -> reduction (app t u) (app r u)
 | reduction_app_r : forall t u r, reduction u r -> reduction (app t u) (app t r)
+| reduction_lft : forall t r, reduction t r -> reduction (lft t) (lft r)
+| reduction_rgt : forall t r, reduction t r -> reduction (rgt t) (rgt r)
+| reduction_cse_e : forall t u1 u2 r, reduction t r -> reduction (cse t u1 u2) (cse r u1 u2)
+| reduction_cse_l : forall t u1 u2 r, reduction u1 r -> reduction (cse t u1 u2) (cse t r u2)
+| reduction_cse_r : forall t u1 u2 r, reduction u2 r -> reduction (cse t u1 u2) (cse t u1 r)
 .
 
 Inductive convertible : term -> term -> Type :=
@@ -63,6 +70,69 @@ transitivity (app t1 u2).
 + apply convertible_app_l; assumption.
 Qed.
 
+Lemma convertible_lft : forall t r,
+  convertible t r -> convertible (lft t) (lft r).
+Proof.
+induction 1.
++ reflexivity.
++ symmetry; assumption.
++ transitivity (lft u); assumption.
++ apply convertible_step, reduction_lft; assumption.
+Qed.
+
+Lemma convertible_rgt : forall t r,
+  convertible t r -> convertible (rgt t) (rgt r).
+Proof.
+induction 1.
++ reflexivity.
++ symmetry; assumption.
++ transitivity (rgt u); assumption.
++ apply convertible_step, reduction_rgt; assumption.
+Qed.
+
+Lemma convertible_cse_e : forall t u1 u2 r,
+  convertible t r -> convertible (cse t u1 u2) (cse r u1 u2).
+Proof.
+induction 1.
++ reflexivity.
++ symmetry; assumption.
++ transitivity (cse u u1 u2); assumption.
++ apply convertible_step, reduction_cse_e; assumption.
+Qed.
+
+Lemma convertible_cse_l : forall t u1 u2 r,
+  convertible u1 r -> convertible (cse t u1 u2) (cse t r u2).
+Proof.
+induction 1.
++ reflexivity.
++ symmetry; assumption.
++ transitivity (cse t u u2); assumption.
++ apply convertible_step, reduction_cse_l; assumption.
+Qed.
+
+Lemma convertible_cse_r : forall t u1 u2 r,
+  convertible u2 r -> convertible (cse t u1 u2) (cse t u1 r).
+Proof.
+induction 1.
++ reflexivity.
++ symmetry; assumption.
++ transitivity (cse t u1 u); assumption.
++ apply convertible_step, reduction_cse_r; assumption.
+Qed.
+
+Lemma convertible_cse : forall t u1 u2 r r1 r2,
+  convertible t r ->
+  convertible u1 r1 ->
+  convertible u2 r2 ->
+  convertible (cse t u1 u2) (cse r r1 r2).
+Proof.
+intros t u1 u2 r r1 r2 H H1 H2.
+etransitivity; [apply convertible_cse_e; eassumption|].
+etransitivity; [apply convertible_cse_l; eassumption|].
+etransitivity; [apply convertible_cse_r; eassumption|].
+reflexivity.
+Qed.
+
 Lemma subs_term_CONS_LFT_n : forall t u e n,
 subs_term (LIFTn n (CONS (lift_term e u) ESID)) (lift_term (ELLFTn n (ELLFT e)) t) =
 lift_term (ELLFTn n e) (subs_term (LIFTn n (CONS u ESID)) t).
@@ -75,6 +145,25 @@ induction t; intros u e m; cbn.
     rewrite lift_compose_ELID_r; reflexivity.
 + f_equal; intuition.
 + f_equal; apply (IHt _ _ (S m)).
++ f_equal; intuition.
++ f_equal; intuition.
++ f_equal; intuition.
+  - apply (IHt2 _ _ (S m)).
+  - apply (IHt3 _ _ (S m)).
+Qed.
+
+Lemma subs_term_LFT_CONS : forall t u e,
+  subs_term (CONS (lift_term e u) ESID) (lift_term (ELLFT e) t) =
+  lift_term e (subs_term (CONS u ESID) t).
+Proof.
+induction t; intros u e; cbn.
+- rewrite !expand_term_CONS; destruct n as [|n]; reflexivity.
+- f_equal; intuition.
+- f_equal.
+  apply subs_term_CONS_LFT_n with (n := 1).
+- f_equal; intuition.
+- f_equal; intuition.
+- f_equal; intuition; apply subs_term_CONS_LFT_n with (n := 1).
 Qed.
 
 Lemma reduction_lift : forall t r e,
@@ -83,19 +172,26 @@ Proof.
 intros t r e Hr; revert e; induction Hr; intros e; cbn in *.
 + evar (r : term); match goal with [ |- reduction _ ?t ] => replace t with r; [refine (reduction_β _ _)|] end;
   unfold r; clear r.
-  revert u e; induction t; intros u e; cbn.
-  - rewrite !expand_term_CONS; destruct n as [|n]; reflexivity.
-  - f_equal; intuition.
-  - f_equal.
-    apply subs_term_CONS_LFT_n with (n := 1).
+  apply subs_term_LFT_CONS.
 + rewrite <- lift_term_compose; cbn.
   rewrite lift_compose_ELID_r.
   replace (lift_term (ELSHFT e) t) with (lift_term (ELSHFT ELID) (lift_term e t)).
   - apply reduction_η.
   - rewrite <- lift_term_compose; reflexivity.
++ evar (r : term); match goal with [ |- reduction _ ?t ] => replace t with r; [refine (reduction_ι_l _ _ _)|] end;
+  unfold r; clear r.
+  apply subs_term_LFT_CONS.
++ evar (r : term); match goal with [ |- reduction _ ?t ] => replace t with r; [refine (reduction_ι_r _ _ _)|] end;
+  unfold r; clear r.
+  apply subs_term_LFT_CONS.
 + apply reduction_lam; intuition.
 + apply reduction_app_l; intuition.
 + apply reduction_app_r; intuition.
++ apply reduction_lft; intuition.
++ apply reduction_rgt; intuition.
++ apply reduction_cse_e; intuition.
++ apply reduction_cse_l; intuition.
++ apply reduction_cse_r; intuition.
 Qed.
 
 Lemma convertible_lift : forall t r e,
