reducibility/NbE_cbv.v
@@ -6,50 +6,89 @@ Require Import Term Convertibility Typing.
 Set Primitive Projections.
 Set Implicit Arguments.
 
-Record eval_atm (Γ : list type) n (t : term) := {
+Record eval_ntr (Γ : list type) A (t : term) := {
   eval_atm_red : term;
-  eval_atm_typ : [ Γ ⊢ne eval_atm_red : atm n ];
+  eval_atm_typ : [ Γ ⊢ne eval_atm_red : A ];
   eval_atm_cnv : convertible t eval_atm_red;
 }.
 
+Definition eval_atm Γ n t := eval_ntr Γ (atm n) t.
+
+Inductive eval_sum evalA evalB Γ A B t :=
+| eval_sum_lft :
+  forall r, evalA r -> convertible t (lft r) -> eval_sum evalA evalB Γ A B t
+| eval_sum_rgt :
+  forall r, evalB r -> convertible t (rgt r) -> eval_sum evalA evalB Γ A B t
+| eval_sum_ntr : eval_ntr Γ (sum A B) t -> eval_sum evalA evalB Γ A B t
+.
+
 Unset Implicit Arguments.
 
-Fixpoint eval (Γ : list type) (A : type) (t : term) : Type :=
+Fixpoint eval (Γ : list type) (A : type) (t : term) {struct A} : Type :=
 match A with
 | atm n => eval_atm Γ n t
 | arr A B =>
   forall Δ (e : lift) (eε : typing_lift e Δ Γ),
   forall (x : term) (xε : eval Δ A x), eval Δ B (app (lift_term e t) x)
+| sum A B => eval_sum (eval Γ A) (eval Γ B) Γ A B t
 end.
 
 Notation realizes := eval.
+
+Lemma lift_eval_ntr : forall Γ Δ A t e, [ Δ ⊢lift e : Γ ] ->
+  eval_ntr Γ A t -> eval_ntr Δ A (lift_term e t).
+Proof.
+intros Γ Δ A t e He Ht.
+destruct Ht as [r Htr Hr]; exists (lift_term e r).
+- apply NF_typing_lift_compat with Γ; assumption.
+- apply convertible_lift; assumption.
+Qed.
 
 Lemma lift_eval : forall Γ Δ A t e, [ Δ ⊢lift e : Γ ] ->
   eval Γ A t -> eval Δ A (lift_term e t).
 Proof.
 intros Γ Δ A; revert Γ Δ; induction A; intros Γ Δ t e He Ht; cbn in *.
-+ destruct Ht as [r Htr Hr]; exists (lift_term e r).
-  - apply NF_typing_lift_compat with Γ; assumption.
-  - apply convertible_lift; assumption.
++ eapply lift_eval_ntr; eassumption.
 + intros Ξ e' He' x xε.
   rewrite <- lift_term_compose.
   apply Ht; [|assumption].
   apply typing_lift_compose with Δ; assumption.
++ destruct Ht as [r Htr Hr|r Htr Hr|Ht].
+  - apply eval_sum_lft with (lift_term e r).
+    { apply IHA1 with Γ; assumption. }
+    { apply convertible_lift with (r := lft _); assumption. }
+  - apply eval_sum_rgt with (lift_term e r).
+    { apply IHA2 with Γ; assumption. }
+    { apply convertible_lift with (r := rgt _); assumption. }
+  - apply eval_sum_ntr; eapply lift_eval_ntr; eassumption.
 Qed.
 
 (* Definition realizes Γ A t := forall Δ (e : lift) (eε : typing_lift e Δ Γ), eval Δ A (lift_term e t). *)
 
+Lemma eval_ntr_convertible_compat : forall Γ A t r, convertible t r -> eval_ntr Γ A t -> eval_ntr Γ A r.
+Proof.
+intros Γ A t r Hr Ht.
+destruct Ht as [s Hs H]; exists s.
+- assumption.
+- apply convertible_trans with t; [|assumption].
+  apply convertible_sym; assumption.
+Qed.
+
 Lemma eval_convertible_compat : forall Γ A t r, convertible t r -> eval Γ A t -> eval Γ A r.
 Proof.
-intros Γ A; revert Γ; induction A as [n|A IHA B IHB]; intros Γ t r Hr Ht; cbn in *.
-+ destruct Ht as [s Hs H]; exists s.
-  - assumption.
-  - apply convertible_trans with t; [|assumption].
-    apply convertible_sym; assumption.
+intros Γ A; revert Γ; induction A as [n|A IHA B IHB|A IHA B IHB]; intros Γ t r Hr Ht; cbn in *.
++ eapply eval_ntr_convertible_compat; eassumption.
 + intros Δ e He x xε.
   apply IHB with (app (lift_term e t) x).
   - apply convertible_app_l, convertible_lift; assumption.
   - apply Ht, xε; assumption.
++ destruct Ht as [s Hts Hs|s Hts Hs|Ht].
+  - apply eval_sum_lft with s; [assumption|].
+    transitivity t; [symmetry|]; assumption.
+  - apply eval_sum_rgt with s; [assumption|].
+    transitivity t; [symmetry|]; assumption.
+  - apply eval_sum_ntr.
+    eapply eval_ntr_convertible_compat; eassumption.
 Qed.
 
 Inductive eval_subs : list type -> list type -> subs term -> Type :=
@@ -58,47 +97,6 @@ Inductive eval_subs : list type -> list type -> subs term -> Type :=
 | eval_subs_SHFT : forall Γ Δ A σ, eval_subs Γ Δ σ -> eval_subs (cons A Γ) Δ (SHFT σ)
 (* | eval_subs_LIFT : forall Γ Δ A σ, eval_subs Γ Δ σ -> eval_subs (cons A Γ) (cons A Δ) (LIFT σ) *)
 .
-
-(* Γ ⊢ t : A -> α ⊩ Γ -> α ⊩ A *)
-Lemma soundness : forall Γ Δ A t σ,
-  [ Γ ⊢ t : A ] -> eval_subs Δ Γ σ -> eval Δ A (subs_term σ t).
-Proof.
-intros Γ Δ A t σ Ht; revert Δ σ; induction Ht; cbn in *; intros Δ σ Hσ.
-+ revert n A e; induction Hσ; intros n B e'; cbn in *.
-  - apply List.nth_error_In in e'; elim e'.
-  - destruct n as [|n]; cbn in *.
-    { injection e'; intros ->; rewrite lift_term_ELID; apply e; constructor. }
-    { apply IHHσ; assumption. }
-  - rewrite expand_term_SHFT.
-    apply lift_eval with Γ; [repeat constructor|].
-    apply IHHσ; assumption.
-+ intros Ξ e eε x xε.
-  eapply eval_convertible_compat; [symmetry; apply convertible_β|].
-  rewrite <- subs_term_lift, <- !subs_term_compose; cbn.
-  apply IHHt. constructor; [assumption|].
-
-  clear - eε Hσ.
-  revert Γ σ Hσ; induction eε; intros Ξ σ Hσ; cbn.
-  - assumption.
-  - constructor; apply IHeε; assumption.
-  - remember (A :: Δ)%list as Ω; revert A Δ eε IHeε HeqΩ; induction Hσ; intros B Ξ eε IHeε HeqΩ; subst.
-    { clear. destruct e; cbn.
-      - change (LIFT (subs_of_lift el)) with (@subs_of_lift term (ELLFT el)); constructor.
-      - rewrite <- subs_lift_compose; do 2 constructor.
-      - rewrite <- subs_lift_compose. refine (eval_subs_ESID _ (ELLFT _)).
-    }
-    { constructor.
-      + change (LIFT (subs_of_lift el)) with (@subs_of_lift term (ELLFT el)).
-        rewrite subs_term_lift; eapply lift_eval; [constructor|]; eassumption.
-      + eapply IHHσ; [eassumption|eassumption|reflexivity]. }
-    { constructor; apply IHeε.
-      injection HeqΩ; intros -> ->; assumption. }
-+ rewrite <- (lift_term_ELID (subs_term σ t)).
-  apply IHHt1 with Δ.
-  - assumption.
-  - constructor.
-  - apply IHHt2; assumption.
-Qed.
 
 Set Implicit Arguments.
 
@@ -151,4 +149,123 @@ induction A; split; cbn in *.
     etransitivity.
     2:{ apply convertible_lam, IHA2.(reify). }
     symmetry; apply convertible_step, reduction_η.
++ intros Γ t Ht.
+  apply eval_sum_ntr; exists t.
+  - assumption.
+  - reflexivity.
++ unshelve refine (@Reified _ _ _ _); cbn.
+  - intros Γ t Ht; cbn in *.
+    destruct Ht as [r Htr Hr|r Htr Hr|[r Htr Hr]].
+    { exact (lft (IHA1.(reify).(reify_trm) _ _ Htr)). }
+    { exact (rgt (IHA2.(reify).(reify_trm) _ _ Htr)). }
+    { refine r. }
+  - intros Γ t Ht; cbn in *.
+    destruct Ht as [r Htr Hr|r Htr Hr|[r Htr Hr]].
+    { apply NF.typing_lft, IHA1.(reify). }
+    { apply NF.typing_rgt, IHA2.(reify). }
+    { apply NF.typing_ne; assumption. }
+  - intros Γ t Ht; cbn in *.
+    destruct Ht as [r Htr Hr|r Htr Hr|[r Htr Hr]]; rewrite Hr.
+    { apply convertible_lft, IHA1.(reify). }
+    { apply convertible_rgt, IHA2.(reify). }
+    { reflexivity. }
+Qed.
+
+Lemma subs_term_CONS_SHFT_LIFT_n : forall t σ n,
+  subs_term (LIFTn n (CONS (var 0) (SHFT σ))) t = subs_term (LIFTn (S n) σ) t.
+Proof.
+induction t; intros σ m; cbn in *; try (solve [f_equal; intuition eauto]).
++ revert n σ; induction m as [|m]; intros n σ; cbn.
+  - rewrite expand_term_CONS, expand_term_LIFT.
+    destruct n as [|n]; [reflexivity|].
+    rewrite expand_term_SHFT; f_equal.
+  - rewrite !expand_term_LIFT; destruct n as [|n]; [reflexivity|]; cbn.
+    f_equal; apply IHm.
++ f_equal; apply (IHt _ (S m)).
++ f_equal; [intuition|apply (IHt2 _ (S m))|apply (IHt3 _ (S m))].
+Qed.
+
+Lemma subs_term_CONS_SHFT_LIFT : forall t σ,
+  subs_term (CONS (var 0) (SHFT σ)) t = subs_term (LIFT σ) t.
+Proof.
+intros t σ; apply subs_term_CONS_SHFT_LIFT_n with (n := 0).
+Qed.
+
+(* Γ ⊢ t : A -> α ⊩ Γ -> α ⊩ A *)
+Lemma soundness : forall Γ Δ A t σ,
+  [ Γ ⊢ t : A ] -> eval_subs Δ Γ σ -> eval Δ A (subs_term σ t).
+Proof.
+intros Γ Δ A t σ Ht; revert Δ σ; induction Ht; cbn in *; intros Δ σ Hσ.
++ revert n A e; induction Hσ; intros n B e'; cbn in *.
+  - apply List.nth_error_In in e'; elim e'.
+  - destruct n as [|n]; cbn in *.
+    { injection e'; intros ->; rewrite lift_term_ELID; apply e; constructor. }
+    { apply IHHσ; assumption. }
+  - rewrite expand_term_SHFT.
+    apply lift_eval with Γ; [repeat constructor|].
+    apply IHHσ; assumption.
++ intros Ξ e eε x xε.
+  eapply eval_convertible_compat; [symmetry; apply convertible_β|].
+  rewrite <- subs_term_lift, <- !subs_term_compose; cbn.
+  apply IHHt. constructor; [assumption|].
+  clear - eε Hσ.
+  revert Γ σ Hσ; induction eε; intros Ξ σ Hσ; cbn.
+  - assumption.
+  - constructor; apply IHeε; assumption.
+  - remember (A :: Δ)%list as Ω; revert A Δ eε IHeε HeqΩ; induction Hσ; intros B Ξ eε IHeε HeqΩ; subst.
+    { clear. destruct e; cbn.
+      - change (LIFT (subs_of_lift el)) with (@subs_of_lift term (ELLFT el)); constructor.
+      - rewrite <- subs_lift_compose; do 2 constructor.
+      - rewrite <- subs_lift_compose. refine (eval_subs_ESID _ (ELLFT _)).
+    }
+    { constructor.
+      + change (LIFT (subs_of_lift el)) with (@subs_of_lift term (ELLFT el)).
+        rewrite subs_term_lift; eapply lift_eval; [constructor|]; eassumption.
+      + eapply IHHσ; [eassumption|eassumption|reflexivity]. }
+    { constructor; apply IHeε.
+      injection HeqΩ; intros -> ->; assumption. }
++ rewrite <- (lift_term_ELID (subs_term σ t)).
+  apply IHHt1 with Δ.
+  - assumption.
+  - constructor.
+  - apply IHHt2; assumption.
++ apply eval_sum_lft with (subs_term σ t).
+  - apply IHHt; assumption.
+  - reflexivity.
++ apply eval_sum_rgt with (subs_term σ t).
+  - apply IHHt; assumption.
+  - reflexivity.
++ destruct (IHHt1 _ _ Hσ) as [r Htr Hr|r Htr Hr|[r Htr Hr]].
+  - eapply eval_convertible_compat.
+    { apply convertible_cse_e; symmetry; eassumption. }
+    eapply eval_convertible_compat; [symmetry; eapply convertible_step, reduction_ι_l|].
+    rewrite <- subs_term_compose; cbn.
+    apply IHHt2; constructor; assumption.
+  - eapply eval_convertible_compat.
+    { apply convertible_cse_e; symmetry; eassumption. }
+    eapply eval_convertible_compat; [symmetry; eapply convertible_step, reduction_ι_r|].
+    rewrite <- subs_term_compose; cbn.
+    apply IHHt3; constructor; assumption.
+  - eapply eval_convertible_compat.
+    shelve.
+    apply (completeness C).(reflect).
+    apply NF.typing_cse with A B.
+    { eexact Htr. }
+    { unshelve apply (completeness C).(reify); [shelve|].
+      apply IHHt2.
+      apply eval_subs_CONS, eval_subs_SHFT, Hσ.
+      apply (completeness A).
+      apply (NF.typing_var _ _ 0); reflexivity. }
+    { unshelve apply (completeness C).(reify); [shelve|].
+      apply IHHt3.
+      apply eval_subs_CONS, eval_subs_SHFT, Hσ.
+      apply (completeness B).
+      apply (NF.typing_var _ _ 0); reflexivity. }
+    Unshelve.
+    apply convertible_cse.
+    { symmetry; assumption. }
+    { rewrite <- (completeness C).(reify).(reify_cvn).
+      rewrite subs_term_CONS_SHFT_LIFT; reflexivity. }
+    { rewrite <- (completeness C).(reify).(reify_cvn).
+      rewrite subs_term_CONS_SHFT_LIFT; reflexivity. }
 Qed.
